work in progress; pointer and positional repr types

src/tls/MITLS.Repr.fst
@@ -38,109 +38,43 @@ module B = LowStar.Buffer
 module HS = FStar.HyperStack
 open FStar.Integers
 module C = LowStar.ConstBuffer
-
-/// A slice is a const uint_8* and a length.
-///
-/// It is a layer around LP.slice, effectively guaranteeing that no
-/// writes are performed via this pointer.
-///
-/// It allows us to uniformly represent `repr t b` backed by either
-/// mutable or immutable arrays.
-noeq
-type const_slice =
-  | MkSlice:
-      base:C.const_buffer LP.byte ->
-      len:uint_32 {
-        UInt32.v len <= C.length base /\
-        len <= LP.validator_max_length
-      } ->
-      const_slice
-
-// When should we use these slices instead of those from LP? Will
-// those definitions eventually go to QD?
-
-[@(deprecated "use const_slice instead")]
-let slice = const_slice
-
-(* Some abbreviations *)
-let mut_p = LowStar.Buffer.trivial_preorder LP.byte
-let immut_p = LowStar.ImmutableBuffer.immutable_preorder LP.byte
-let preorder (c:const_slice) = C.qbuf_pre (C.as_qbuf c.base)
-
-let live h (b:const_slice) = LowStar.ConstBuffer.live h b.base
-let loc (b:const_slice) = LowStar.ConstBuffer.loc_buffer b.base
-let as_seq h (b:const_slice) = LowStar.ConstBuffer.as_seq h b.base
-
-(* conversion between LP.slices and const_slices *)
-let of_slice (x:LP.slice mut_p mut_p { LP.(x.len <= LP.validator_max_length) })
-  : Tot const_slice
-  = MkSlice (C.of_buffer LP.(x.base)) LP.(x.len)
-
-let of_islice (x:LP.slice immut_p immut_p { LP.(x.len <= LP.validator_max_length) })
-  : Tot const_slice
-  = MkSlice (C.of_ibuffer LP.(x.base)) LP.(x.len)
-
-let to_slice (x:const_slice)
-  : Tot (LP.slice (preorder x) (preorder x))
-  = let b = C.cast x.base in
-    let len = x.len in
-    LP.({
-       base = b;
-       len = len
-    })
+include LowParse.Ptr
+module Ptr = LowParse.Ptr
 
 /// `index b` is the type of valid indexes into `b`
-let index (b:const_slice)= i:uint_32{ i <= b.len }
+let index (b:const_slice)= i:uint_32{ i <= b.slice_len }
 
-/// `strong_parser_kind`: We restrict our attention to the
-/// representation of types whose parsers have the strong-prefix
-/// property.
-let strong_parser_kind =
-    k:LP.parser_kind{
-      LP.(k.parser_kind_subkind == Some ParserStrong)
-    }
-
-
+module U32 = FStar.UInt32
 (*** Representation types ***)
-
-/// `repr_meta t`: Each representation is associated with
-/// specification metadata that records
-///
-///  -- the parser(s) that defines its wire format
-///  -- the represented value
-///  -- the bytes of its wire format
-noeq
-type repr_meta (t:Type) = {
-  parser_kind: strong_parser_kind;
-  parser:LP.parser parser_kind t;
-  parser32:LS.parser32 parser;
-  v: t;
-  repr_bytes: Seq.seq LP.byte
-}
-// is it a good use case for `erasable` ?
-// why keeping repr_bytes + invariant vs recalculating it from v?
-
-/// `repr t b`: The main type of this module.
-///
-///   * The slice `b` holds a representation of `t` in
-///    `b.[start_pos, end_pos)`
-///
-///   * The representation is described by erased the `meta` field
-///
-///   * At this stage, we also keep a real high-level value (vv). We
-///     plan to gradually access instead its ghost (.meta.v) and
-///     eventually get rid of it to lower implicit heap allocations.
-///
-///   * Similarly, we should consider passing fewer real indexes
-///     around: we need access to start_pos, but probably not to
-///     end_pos (recomputable anyway) or b.len.
 noeq
 type repr (t:Type) (b:const_slice) = {
   start_pos: index b;
-  end_pos: i:index b {start_pos <= i /\ i <= b.len};
-  meta: Ghost.erased (repr_meta t);
-  vv: x:t{x == (Ghost.reveal meta).v}
+  meta:meta t;
+  value: t;
+  meta_ok:squash (U32.v start_pos + U32.v meta.len <= U32.v b.slice_len /\
+                  value == meta.v)
 }
+
+open FStar.HyperStack.ST
+
+/// This is a variant of `sub` that takes an erased `len`
+/// Should be able to add this to the buffer model
+/// If not, we can use the `offset` function, which is less precise
+assume
+val sub (c:C.const_buffer 'a) (i:uint_32) (len:Ghost.erased uint_32)
+  : Stack (C.const_buffer 'a)
+    (requires fun h ->
+      C.live h c /\
+      U32.v i + U32.v (Ghost.reveal len) <= C.length c)
+    (ensures fun h0 c' h1 ->
+      let qc = C.as_qbuf c in
+      let qc' = C.as_qbuf c' in
+      h0 == h1 /\
+      c' `C.const_sub_buffer i (Ghost.reveal len)` c)
+
+let const_buffer_of_repr #t #b (r:repr t b)
+  : GTot (C.const_buffer LP.byte)
+  = C.gsub b.base r.start_pos r.meta.len
 
 
 /// `repr_p`
@@ -155,45 +89,22 @@ type repr (t:Type) (b:const_slice) = {
 /// representations from wire formats. At those points, the `repr_p`
 /// type is useful, since it is a `repr` that is also indexed by a
 /// parser.
-let repr_p (t:Type) (b:const_slice) #k (#parser:LP.parser k t) (parser32:LS.parser32 parser) =
+let repr_p (t:Type) (b:const_slice) #k (parser:LP.parser k t) =
   r:repr t b {
-    let meta = Ghost.reveal r.meta in
-    meta.parser_kind == k /\
-    meta.parser == parser /\
-    meta.parser32 == parser32
+    r.meta.parser_kind == k /\
+    r.meta.parser == parser
   }
-// No harm in passing parser32, even if it is seldom used.
 
 (*** Validity ***)
-
-/// `valid' r h`:
-///   We define validity in two stages:
-///
-///   First, we provide `valid'`, a transparent definition and then
-///   turn it `abstract` by the `valid` predicate just below.
-///
-///   Validity encapsulates three related LowParse properties:notions:
-///
-///    1. The underlying slice contains a valid wire-format
-///    (`valid_pos`)
-///
-///    2. The ghost value associated with the `repr` is the
-///    parsed value of the wire format.
-///
-///    3. The bytes of the slice are indeed the representation of the
-///    ghost value in wire format
+/// we just inherited the validity from pointers
 let valid' (#t:Type) (#b:const_slice) (r:repr t b) (h:HS.mem)
-  = let m = Ghost.reveal r.meta in
-    let b = to_slice b in
-    LP.valid_pos m.parser h b r.start_pos r.end_pos /\
-    m.v == LP.contents m.parser h b r.start_pos /\
-    m.repr_bytes == LP.bytes_of_slice_from_to h b r.start_pos r.end_pos
+  = let b = to_slice (Ptr.MkSlice (const_buffer_of_repr r) r.meta.len) in
+    Ptr.valid_slice b r.meta h
 
 /// `valid`: abstract validity
 abstract
 let valid (#t:Type) (#b:const_slice) (r:repr t b) (h:HS.mem)
   = valid' r h
-
 
 /// `reveal_valid`:
 ///   An explicit lemma exposes the definition of `valid`
@@ -207,7 +118,7 @@ let reveal_valid ()
 ///         sub-slice b.[from, to)
 let fp #t (#b:const_slice) (r:repr t b)
   : GTot B.loc
-  = LP.loc_slice_from_to (to_slice b) r.start_pos r.end_pos
+  = C.loc_buffer (const_buffer_of_repr r)
 
 /// `frame_valid`:
 ///    A framing principle for `valid r h`
@@ -222,36 +133,49 @@ let frame_valid #t #b (r:repr t b) (l:B.loc) (h0 h1:HS.mem)
       valid r h1)
     [SMTPat (valid r h1);
      SMTPat (B.modifies l h0 h1)]
-  = B.modifies_buffer_from_to_elim LP.((to_slice b).base) r.start_pos r.end_pos l h0 h1
+  = ()
 
+(*** Operations on reprs ***)
 
-/// `value`: A convenience function to access the underlying value
-/// represented
-let value #t #b (r:repr t b)
-  : GTot t
-  = (Ghost.reveal r.meta).v
-// do we use `repr` in other libraries for it :) ? maybe reserve `v`
-// for this one if it is pervasive in e.g. Machine?
-
-open FStar.HyperStack.ST
-
-/// `to_bytes`: for intermediate purposes only, extract bytes from the repr
-let to_bytes #t #b (r: repr t b)
-  : Stack FStar.Bytes.bytes
+/// Mostly just by inheriting operations on pointers
+let as_ptr #t #b (r:repr t b)
+  : Stack (ptr t)
     (requires fun h ->
-      valid r h
-    )
-    (ensures fun h x h' ->
-      B.modifies B.loc_none h h' /\
-      FStar.Bytes.reveal x == (Ghost.reveal r.meta).repr_bytes /\
-      FStar.Bytes.len x == r.end_pos - r.start_pos
-    )
-  = let len = r.end_pos - r.start_pos in
-    let b' = C.sub b.base r.start_pos len in
-    (* FIXME: FStar.Bytes does not cater to const buffers,
-       but do we really care, this code is transitional anyway *)
-    assume (C.qbuf_qual (C.as_qbuf b') == C.MUTABLE);
-    FStar.Bytes.of_buffer len (C.cast b')
+      LP.live_slice h (to_slice b))
+    (ensures fun h0 ptr h1 ->
+      ptr.b `C.const_sub_buffer r.start_pos r.meta.len` b.base /\
+      ptr.Ptr.meta == r.meta /\
+      h0 == h1 /\
+      (valid r h1 <==> Ptr.valid ptr h1))
+  = let b = sub b.base r.start_pos (Ghost.hide r.meta.len) in
+    let m = r.meta in
+    let v = r.value in
+    let open Ptr in
+    let p =
+      { b = b;
+        meta = m;
+        value = v;
+        ptr_ok = ()}
+    in
+    Ptr.reveal_valid ();
+    p
+
+let as_repr #t (b:const_slice) (from to:index b) (p:ptr t)
+  : Pure (repr t b)
+    (requires
+      from <= to /\
+      p.Ptr.b == C.gsub b.base from (to - from))
+    (ensures fun r ->
+      (forall h. Ptr.valid p h <==> valid r h))
+  = Ptr.reveal_valid();
+    {
+      start_pos = from;
+      meta = p.Ptr.meta;
+      value = p.Ptr.value;
+      meta_ok = ()
+    }
+
+
 
 /// `mk b from to p`:
 ///    Constructing a `repr` from a sub-slice
@@ -262,87 +186,35 @@ let mk (b:LP.slice mut_p mut_p{ LP.(b.len <= validator_max_length) })
        (from to:index (of_slice b))
        (#k:strong_parser_kind) #t (#parser:LP.parser k t)
        (parser32:LS.parser32 parser)
-  : Stack (repr_p t (of_slice b) parser32)
+  : Stack (repr_p t (of_slice b) parser)
     (requires fun h ->
       LP.valid_pos parser h b from to)
     (ensures fun h0 r h1 ->
       B.(modifies loc_none h0 h1) /\
       valid r h1 /\
       r.start_pos = from /\
-      r.end_pos = to /\
-      value r == LP.contents parser h1 b from)
-  = let h = get () in
-    let m =
-      let v = LP.contents parser h b from in
-      Ghost.hide ({
-        parser_kind = _;
-        parser = parser;
-        parser32 = parser32;
-        v = v;
-        repr_bytes = LP.bytes_of_slice_from_to h b from to
-      })
-    in
-
-    LP.contents_exact_eq parser h b from to;
-
-    // Compute [.vv]; this code will eventually disappear
-    let sub_b = B.sub b.LP.base from (to - from) in
-    let sub_b_bytes = FStar.Bytes.of_buffer (to - from) sub_b in
-    match parser32 sub_b_bytes with
-    | Some (v, _) ->
-      {
-        start_pos = from;
-        end_pos = to;
-        vv = v;
-        meta = m
-      }
+      r.value == LP.contents parser h1 b from)
+  = as_repr (of_slice b) from to (Ptr.mk b from to parser32)
 
 /// `mk b from to p`:
 ///    Constructing a `repr` from a sub-slice
 ///      b.[from, to)
 ///    known to be valid for a given wire-format parser `p`
-#set-options "--z3rlimit 20"
 inline_for_extraction
 let mk_from_const_slice
          (b:const_slice)
          (from to:index b)
          (#k:strong_parser_kind) #t (#parser:LP.parser k t)
          (parser32:LS.parser32 parser)
-  : Stack (repr_p t b parser32)
+  : Stack (repr_p t b parser)
     (requires fun h ->
       LP.valid_pos parser h (to_slice b) from to)
     (ensures fun h0 r h1 ->
       B.(modifies loc_none h0 h1) /\
       valid r h1 /\
       r.start_pos = from /\
-      r.end_pos = to /\
-      value r == LP.contents parser h1 (to_slice b) from)
-  = let h = get () in
-    assume (C.qbuf_qual (C.as_qbuf b.base) == C.MUTABLE);
-    let b = to_slice b in
-    let m =
-      let v = LP.contents parser h b from in
-      Ghost.hide ({
-        parser_kind = _;
-        parser = parser;
-        parser32 = parser32;
-        v = v;
-        repr_bytes = LP.bytes_of_slice_from_to h b from to
-      })
-    in
-
-    LP.contents_exact_eq parser h b from to;
-
-    let sub_b = B.sub b.LP.base from (to - from) in
-    let sub_b_bytes = FStar.Bytes.of_buffer (to - from) sub_b in
-    match parser32 sub_b_bytes with
-    | Some (v, _) ->
-      {
-        start_pos = from;
-        end_pos = to;
-        vv = v;
-        meta = m
-      }
+      r.value == LP.contents parser h1 (to_slice b) from)
+  = as_repr b from to (Ptr.mk_from_const_slice b from to parser32)
 
 /// A high-level constructor, taking a value instead of a slice.
 ///
@@ -357,7 +229,7 @@ let mk_from_serialize
   (#k:strong_parser_kind) #t (#parser:LP.parser k t) (#serializer: LP.serializer parser)
   (parser32: LS.parser32 parser) (serializer32: LS.serializer32 serializer)
   (size32: LS.size32 serializer) (x: t)
-: Stack (option (repr_p t (of_slice b) parser32))
+: Stack (option (repr_p t (of_slice b) parser))
     (requires fun h ->
       LP.live_slice h b)
     (ensures fun h0 r h1 ->
@@ -369,162 +241,10 @@ let mk_from_serialize
       | Some r ->
         valid r h1 /\
         r.start_pos == from /\
-        value r == x
+        r.value == x
       end
     )
 = let size = size32 x in
-  let len = b.LP.len - from in
-  if len < size
-  then None
-  else begin
-    let bytes = serializer32 x in
-    let dst = B.sub b.LP.base from size in
-    (if size > 0ul then FStar.Bytes.store_bytes bytes dst);
-    let to = from + size in
-    let h = get () in
-    LP.serialize_valid_exact serializer h b x from to;
-    let r = mk b from to parser32 in
-    Some r
-  end
-
-(*** Stable Representations ***)
-
-(*
-   By copying a representation into an immutable buffer `i`,
-   we obtain a stable representation, which remains valid so long
-   as the `i` remains live.
-
-   We achieve this by relying on support for monotonic state provided
-   by Low*, as described in the POPL '18 paper "Recalling a Witness"
-
-   TODO: The feature also relies on an as yet unimplemented feature to
-         atomically allocate and initialize a buffer to a chosen
-         value. This will soon be added to the LowStar library.
-*)
-
-module I = LowStar.ImmutableBuffer
-
-/// `valid_if_live`: A pure predicate on `r:repr t b` that states that
-/// so long as the underlying buffer is live in a given state `h`,
-/// `r` is valid in that state
-let valid_if_live #t (#b:const_slice) (r:repr t b) =
-  C.qbuf_qual (C.as_qbuf b.base) == C.IMMUTABLE /\
-  (let i : I.ibuffer LP.byte = C.as_mbuf b.base in
-   let m = Ghost.reveal r.meta in
-   exists (h:HS.mem).{:pattern valid r h}
-      i `I.value_is` Ghost.hide m.repr_bytes /\
-      m.repr_bytes == B.as_seq h i /\
-      valid r h /\
-      (forall h'.
-        C.live h' b.base /\
-        B.as_seq h i `Seq.equal` B.as_seq h' i ==>
-        valid r h'))
-
-/// `stable_repr t b`: A representation that is valid if its buffer is
-/// live
-let stable_repr t b = r:repr t b { valid_if_live r }
-
-/// `valid_if_live_intro` :
-///    An internal lemma to introduce `valid_if_live`
-
-// Note: the next proof is flaky and occasionally enters a triggering
-// vortex with the notorious FStar.Seq.Properties.slice_slice
-// Removing that from the context makes the proof instantaneous
-#reset-options "--max_fuel 0 --max_ifuel 0 \
-                --using_facts_from '* -FStar.Seq.Properties.slice_slice'"
-let valid_if_live_intro #t (#b:const_slice) (r:repr t b) (h:HS.mem)
-  : Lemma
-    (requires (
-      C.qbuf_qual (C.as_qbuf b.base) == C.IMMUTABLE /\
-      valid r h /\
-      (let i : I.ibuffer LP.byte = C.as_mbuf b.base in
-       let m = Ghost.reveal r.meta in
-       B.as_seq h i == m.repr_bytes /\
-       i `I.value_is` Ghost.hide m.repr_bytes)))
-    (ensures
-      valid_if_live r)
-  = let i : I.ibuffer LP.byte = C.as_mbuf b.base in
-    let aux (h':HS.mem)
-        : Lemma
-          (requires
-            C.live h' b.base /\
-            B.as_seq h i `Seq.equal` B.as_seq h' i)
-          (ensures
-            valid r h')
-          [SMTPat (valid r h')]
-        = let m = Ghost.reveal r.meta in
-          LP.valid_ext_intro m.parser h (to_slice b) r.start_pos h' (to_slice b) r.start_pos
-    in
-    ()
-
-/// `recall_stable_repr` Main lemma: if the underlying buffer is live
-///    then a stable repr is valid
-let recall_stable_repr #t #b (r:stable_repr t b)
-  : Stack unit
-    (requires fun h ->
-      C.live h b.base)
-    (ensures fun h0 _ h1 ->
-      h0 == h1 /\
-      valid r h1)
-  = let h1 = get () in
-    let i = C.to_ibuffer b.base in
-    let aux (h:HS.mem)
-      : Lemma
-        (requires
-          valid r h /\
-          B.as_seq h i == B.as_seq h1 i)
-        (ensures
-          valid r h1)
-        [SMTPat (valid r h)]
-      = let m = Ghost.reveal r.meta in
-        LP.valid_ext_intro m.parser h (to_slice b) r.start_pos h1 (to_slice b) r.start_pos
-     in
-     let es =
-       let m = Ghost.reveal r.meta in
-       Ghost.hide m.repr_bytes
-     in
-     I.recall_value i es
-
-/// `stash`: Main stateful operation
-///    Copies a repr into a fresh stable repr
-let stash (rgn:HS.rid) #t #b (r:repr t b)
-  : ST (s:const_slice &
-        r':stable_repr t s)
-   (requires fun h ->
-     valid r h)
-   (ensures fun h0 (|s, r'|) h1 ->
-     B.modifies B.loc_none h0 h1 /\
-     valid r' h1 /\
-     r.meta == r'.meta)
-     //Add that the slice s is actually in region rgn
-     //And that the slice is live if the region is live
- = let r_len = r.end_pos - r.start_pos in
-   let b_sub = C.sub b.base r.start_pos r_len in
-   (*
-    * AR: Should this be a precondition?
-    *)
-   assume (is_eternal_region rgn);
-   (*
-    * AR: Allocation functions in the buffer library require r_len > 0
-    *     Should we maintain anyway that in a repr end_pos > start_pos?
-    *)
-   assume (r_len > 0ul);
-   let buf' = I.igcmalloc_and_blit rgn (C.cast b_sub) 0ul r_len in
-   let s = MkSlice (C.of_ibuffer buf') r_len in
-   let h1 = get () in
-   let _ =
-     let m = Ghost.reveal r.meta in
-     assert (LP.valid_pos m.parser h1 (to_slice b) r.start_pos r.end_pos)    ;
-     LP.valid_ext_intro m.parser h1 (to_slice b) r.start_pos h1 (to_slice s) 0ul;
-     assert (LP.valid_pos m.parser h1 (to_slice s) 0ul r_len)
-   in
-   let r' : repr t s = {
-     start_pos = 0ul;
-     end_pos = r_len;
-     meta = r.meta;
-     vv = r.vv
-   }
-   in
-   assert (valid r' h1);
-   valid_if_live_intro r' h1;
-   (| s, r' |)
+  match (mk_from_serialize b from parser32 serializer32 size32 x) with
+  | None -> None
+  | Some p -> Some (as_repr (of_slice b) from (from + size) p)
