src/tls/LowParse.Ptr.fst
@@ -1,0 +1,497 @@
+(*
+  Copyright 2015--2019 INRIA and Microsoft Corporation
+
+  Licensed under the Apache License, Version 2.0 (the "License");
+  you may not use this file except in compliance with the License.
+  You may obtain a copy of the License at
+
+    http://www.apache.org/licenses/LICENSE-2.0
+
+  Unless required by applicable law or agreed to in writing, software
+  distributed under the License is distributed on an "AS IS" BASIS,
+  WITHOUT WARRANTIES OR CONDITIONS OF ANY KIND, either express or implied.
+  See the License for the specific language governing permissions and
+  limitations under the License.
+
+  Authors: T. Ramananandro, A. Rastogi, N. Swamy, A. Fromherz
+*)
+module LowParse.Ptr
+
+module LP = LowParse.Low.Base
+module LS = LowParse.SLow.Base
+module B = LowStar.Buffer
+module HS = FStar.HyperStack
+module C = LowStar.ConstBuffer
+module U32 = FStar.UInt32
+open FStar.Integers
+open FStar.HyperStack.ST
+
+(* Summary:
+
+   A pointer-based representation type.
+
+   See https://github.com/mitls/mitls-papers/wiki/The-Memory-Model-of-miTLS#pointer-based-transient-reprs
+
+   Calling it LowParse.Ptr since it should eventually move to everparse/src/lowparse
+ *)
+
+/// `strong_parser_kind`: We restrict our attention to the
+/// representation of types whose parsers have the strong-prefix
+/// property.
+let strong_parser_kind =
+    k:LP.parser_kind{
+      LP.(k.parser_kind_subkind == Some ParserStrong)
+    }
+
+let preorder (c:C.const_buffer LP.byte) = C.qbuf_pre (C.as_qbuf c)
+
+let slice_of_const_buffer (b:C.const_buffer LP.byte) (len:uint_32{U32.v len <= C.length b}) 
+  : LP.slice (preorder b) (preorder b)
+  = let b = C.cast b in
+    LP.({
+       base = b;
+       len = len
+    })
+
+let mut_p = LowStar.Buffer.trivial_preorder LP.byte
+
+(*** Representation types ***)
+
+/// `meta t`: Each representation is associated with
+/// specification metadata that records
+///
+///  -- the parser(s) that defines its wire format
+///  -- the represented value
+///  -- the bytes of its wire format
+/// 
+///  We retain both the value and its wire format for convenience.
+/// 
+///  An alternative would be to also retain here a serializer and then
+///  compute the bytes when needed from the serializer. But that's a
+///  bit heavy
+[@erasable]
+noeq
+type meta (t:Type) = {
+  parser_kind: strong_parser_kind;
+  parser:LP.parser parser_kind t;
+  parser32:LS.parser32 parser;
+  v: t;
+  len: uint_32;
+  repr_bytes: Seq.lseq LP.byte (U32.v len);
+  meta_ok: squash (LowParse.Spec.Base.parse parser repr_bytes == Some (v, U32.v len))
+}
+
+/// `ptr t`: The main type of this module.
+///
+///   * The const pointer `b` refers to a representation of `t`
+///
+///   * The representation is described by erased the `meta` field
+///
+///   * At this stage, we also keep a real high-level value (vv). We
+///     plan to gradually access instead its ghost (.meta.v) and
+///     eventually get rid of it to lower implicit heap allocations.
+noeq
+type ptr (t:Type) = {
+  b : C.const_buffer LP.byte;
+  meta: meta t;
+  value: t;
+  ptr_ok: squash (U32.v meta.len == C.length b /\
+                  value == meta.v)
+}
+
+let ptr_p (t:Type) (#k:strong_parser_kind) (parser:LP.parser k t) =
+  p:ptr t{ p.meta.parser_kind == k /\ p.meta.parser == parser }
+
+let slice_of_ptr #t (p:ptr t) 
+  : GTot (LP.slice (preorder p.b) (preorder p.b))
+  = slice_of_const_buffer p.b p.meta.len
+
+(*** Validity ***)
+
+/// `valid' r h`:
+///   We define validity in two stages:
+///
+///   First, we provide `valid'`, a transparent definition and then
+///   turn it `abstract` by the `valid` predicate just below.
+///
+///   Validity encapsulates three related LowParse properties:notions:
+///
+///    1. The underlying pointer contains a valid wire-format
+///    (`valid_pos`)
+///
+///    2. The ghost value associated with the `repr` is the
+///        parsed value of the wire format.
+///
+///    3. The bytes of the slice are indeed the representation of the
+///       ghost value in wire format
+unfold 
+let valid_slice (#t:Type) (#r #s:_) (slice:LP.slice r s) (meta:meta t) (h:HS.mem) =
+  LP.valid_pos meta.parser h slice 0ul meta.len /\
+  meta.repr_bytes == LP.bytes_of_slice_from_to h slice 0ul meta.len
+
+unfold 
+let valid' (#t:Type) (p:ptr t) (h:HS.mem) =
+  let slice = slice_of_const_buffer p.b p.meta.len in
+  valid_slice slice p.meta h
+
+/// `valid`: abstract validity
+abstract
+let valid (#t:Type) (p:ptr t) (h:HS.mem)
+  = valid' p h
+
+/// `reveal_valid`:
+///   An explicit lemma exposes the definition of `valid`
+let reveal_valid ()
+  : Lemma (forall (t:Type) (p:ptr t) (h:HS.mem).
+              {:pattern (valid #t p h)}
+           valid #t p h <==> valid' #t p h)
+  = ()
+
+/// `fp r`: The memory footprint of a ptr is the underlying pointer
+let fp #t (p:ptr t)
+  : GTot B.loc
+  = C.loc_buffer p.b
+
+/// `frame_valid`:
+///    A framing principle for `valid r h`
+///    It is invariant under footprint-preserving heap updates
+let frame_valid #t (p:ptr t) (l:B.loc) (h0 h1:HS.mem)
+  : Lemma
+    (requires
+      valid p h0 /\
+      B.modifies l h0 h1 /\
+      B.loc_disjoint (fp p) l)
+    (ensures
+      valid p h1)
+    [SMTPat (valid p h1);
+     SMTPat (B.modifies l h0 h1)]
+  = ()
+
+(***  Contructors ***)
+
+
+/// A slice is a const uint_8* and a length.
+///
+/// It is a layer around LP.slice, effectively guaranteeing that no
+/// writes are performed via this pointer.
+///
+/// It allows us to uniformly represent `ptr t` backed by either
+/// mutable or immutable arrays.
+noeq
+type const_slice =
+  | MkSlice:
+      base:C.const_buffer LP.byte ->
+      slice_len:uint_32 {
+        UInt32.v slice_len <= C.length base /\
+        slice_len <= LP.validator_max_length
+      } ->
+      const_slice
+
+let to_slice (x:const_slice)
+  : Tot (LP.slice (preorder x.base) (preorder x.base))
+  = let b = C.cast x.base in
+    let len = x.slice_len in
+    LP.({
+       base = b;
+       len = len
+    })
+
+let of_slice (x:LP.slice mut_p mut_p {x.LP.len <= LP.validator_max_length} )
+  : Tot const_slice
+  = let b = C.of_buffer x.LP.base in
+    let len = x.LP.len in
+    MkSlice b len
+    
+assume
+val of_mbuffer: #p:_ -> #q:_ -> l:UInt32.t -> buf:B.mbuffer LP.byte p q -> Stack (b:FStar.Bytes.bytes{FStar.Bytes.length b = UInt32.v l})
+  (requires (fun h0 -> B.live h0 buf))
+  (ensures  (fun h0 b h1 -> B.(modifies loc_none h0 h1) /\ b = FStar.Bytes.hide (B.as_seq h0 buf)))
+
+/// `mk b from to p`:
+///    Constructing a `ptr` from a sub-slice
+///      b.[from, to)
+///    known to be valid for a given wire-format parser `p`
+#set-options "--z3rlimit 20"
+inline_for_extraction
+let mk_from_const_slice
+         (b:const_slice)
+         (from to:uint_32)
+         (#k:strong_parser_kind) #t (#parser:LP.parser k t)
+         (parser32:LS.parser32 parser)
+  : Stack (ptr_p t parser)
+    (requires fun h ->
+      LP.valid_pos parser h (to_slice b) from to)
+    (ensures fun h0 p h1 ->
+      B.(modifies loc_none h0 h1) /\
+      valid p h1 /\
+      p.meta.v == LP.contents parser h1 (to_slice b) from /\
+      p.b `C.const_sub_buffer from (to - from)` b.base)
+  = let h = get () in
+    let slice = to_slice b in
+    LP.contents_exact_eq parser h slice from to;    
+    let meta :meta t = {
+        parser_kind = _;
+        parser = parser;
+        parser32 = parser32;
+        v = LP.contents parser h slice from;
+        len = to - from;
+        repr_bytes = LP.bytes_of_slice_from_to h slice from to;
+        meta_ok = ()
+    } in 
+    let sub_b = C.sub b.base from (to - from) in
+    let value = 
+      // Compute [.v]; this code will eventually disappear
+      let sub_b_bytes = of_mbuffer (to - from) (C.cast sub_b) in
+      let Some (v, _) = parser32 sub_b_bytes in
+      v
+    in
+    let p = {
+      b = sub_b;
+      meta = meta;
+      value = value;
+      ptr_ok = ()
+    } in
+    let h1 = get () in
+    let slice' = slice_of_const_buffer sub_b (to - from) in
+    LP.valid_facts p.meta.parser h1 slice from; //elim valid_pos slice
+    LP.valid_facts p.meta.parser h1 slice' 0ul; //intro valid_pos slice'
+    p
+
+/// `mk b from to p`:
+///    Constructing a `ptr` from a LowParse slice
+///      b.[from, to)
+///    known to be valid for a given wire-format parser `p`
+inline_for_extraction
+let mk (slice:LP.slice mut_p mut_p{ slice.LP.len <= LP.validator_max_length })
+       (from to:uint_32)
+       (#k:strong_parser_kind) #t (#parser:LP.parser k t)
+       (parser32:LS.parser32 parser)
+  : Stack (ptr_p t parser)
+    (requires fun h ->
+      LP.valid_pos parser h slice from to)
+    (ensures fun h0 p h1 ->
+      B.(modifies loc_none h0 h1) /\
+      valid p h1 /\
+      p.b `C.const_sub_buffer from (to - from)` (C.of_buffer slice.LP.base) /\
+      p.meta.v == LP.contents parser h1 slice from)
+  = let c = MkSlice (C.of_buffer slice.LP.base) slice.LP.len in
+    mk_from_const_slice c from to parser32
+
+/// A high-level constructor, taking a value instead of a slice.
+///
+/// Can we remove the `noextract` for the time being? Can we
+/// `optimize` it so that vv is assigned x? It will take us a while to
+/// lower all message writing.
+inline_for_extraction
+noextract
+let mk_from_serialize
+    (b:LP.slice mut_p mut_p{ LP.(b.len <= validator_max_length) })
+    (from:uint_32 { from <= b.LP.len })
+    (#k:strong_parser_kind) #t (#parser:LP.parser k t) (#serializer: LP.serializer parser)
+    (parser32: LS.parser32 parser) (serializer32: LS.serializer32 serializer)
+    (size32: LS.size32 serializer) (x: t)
+  : Stack (option (ptr_p t parser))
+    (requires fun h ->
+       LP.live_slice h b)
+    (ensures fun h0 popt h1 ->
+       B.modifies (LP.loc_slice_from b from) h0 h1 /\
+       (match popt with
+       | None ->
+         (* not enough space in output slice *)
+         Seq.length (LP.serialize serializer x) > FStar.UInt32.v (b.LP.len - from)
+       | Some p ->
+         let size = size32 x in
+         valid p h1 /\
+         U32.v from + U32.v size <= U32.v b.LP.len /\
+         p.b == C.gsub (C.of_buffer b.LP.base) from size /\
+         p.meta.v == x))
+  = let size = size32 x in
+    let len = b.LP.len - from in
+    if len < size
+    then None
+    else begin
+      let bytes = serializer32 x in
+      let dst = B.sub b.LP.base from size in
+      (if size > 0ul then FStar.Bytes.store_bytes bytes dst);
+        let to = from + size in
+      let h = get () in
+      LP.serialize_valid_exact serializer h b x from to;
+      let r = mk b from to parser32 in
+      Some r
+    end
+
+(*** Destructors ***)
+
+/// `to_bytes`: for intermediate purposes only, extract bytes from the repr
+let to_bytes #t (p: ptr t) (len:uint_32)
+  : Stack FStar.Bytes.bytes
+    (requires fun h ->
+      valid p h /\
+      len == p.meta.len
+    )
+    (ensures fun h x h' ->
+      B.modifies B.loc_none h h' /\
+      FStar.Bytes.reveal x == p.meta.repr_bytes /\
+      FStar.Bytes.len x == p.meta.len
+    )
+  = of_mbuffer len (C.cast p.b)
+
+
+(*** Stable Representations ***)
+
+(*
+   By copying a representation into an immutable buffer `i`,
+   we obtain a stable representation, which remains valid so long
+   as the `i` remains live.
+
+   We achieve this by relying on support for monotonic state provided
+   by Low*, as described in the POPL '18 paper "Recalling a Witness"
+
+   TODO: The feature also relies on an as yet unimplemented feature to
+         atomically allocate and initialize a buffer to a chosen
+         value. This will soon be added to the LowStar library.
+*)
+
+module I = LowStar.ImmutableBuffer
+
+/// `valid_if_live`: A pure predicate on `r:ptr t` that states that
+/// so long as the underlying buffer is live in a given state `h`,
+/// `p` is valid in that state
+let valid_if_live #t (p:ptr t) =
+  C.qbuf_qual (C.as_qbuf p.b) == C.IMMUTABLE /\
+  (let i : I.ibuffer LP.byte = C.as_mbuf p.b in
+   let m = p.meta in
+   exists (h:HS.mem).{:pattern valid p h}
+      i `I.value_is` Ghost.hide m.repr_bytes /\
+      m.repr_bytes == B.as_seq h i /\
+      valid p h /\
+      (forall h'.
+        C.live h' p.b /\
+        B.as_seq h i `Seq.equal` B.as_seq h' i ==>
+        valid p h'))
+
+/// `stable_ptr t`: A representation that is valid if its buffer is
+/// live
+let stable_ptr t= p:ptr t { valid_if_live p }
+
+/// `valid_if_live_intro` :
+///    An internal lemma to introduce `valid_if_live`
+
+// Note: the next proof is flaky and occasionally enters a triggering
+// vortex with the notorious FStar.Seq.Properties.slice_slice
+// Removing that from the context makes the proof instantaneous
+#push-options "--max_ifuel 1 --initial_ifuel 1 \
+                --using_facts_from '* -FStar.Seq.Properties.slice_slice'"
+let valid_if_live_intro #t (r:ptr t) (h:HS.mem)
+  : Lemma
+    (requires (
+      C.qbuf_qual (C.as_qbuf r.b) == C.IMMUTABLE /\
+      valid r h /\
+      (let i : I.ibuffer LP.byte = C.as_mbuf r.b in
+       let m = r.meta in
+       B.as_seq h i == m.repr_bytes /\
+       i `I.value_is` Ghost.hide m.repr_bytes)))
+    (ensures
+      valid_if_live r)
+  = let i : I.ibuffer LP.byte = C.as_mbuf r.b in
+    let aux (h':HS.mem)
+        : Lemma
+          (requires
+            C.live h' r.b /\
+            B.as_seq h i `Seq.equal` B.as_seq h' i)
+          (ensures
+            valid r h')
+          [SMTPat (valid r h')]
+        = let m = r.meta in
+          LP.valid_ext_intro m.parser h (slice_of_ptr r) 0ul h' (slice_of_ptr r) 0ul
+    in
+    ()
+
+/// `recall_stable_ptr` Main lemma: if the underlying buffer is live
+///    then a stable ptr is valid
+let recall_stable_ptr #t (r:stable_ptr t)
+  : Stack unit
+    (requires fun h ->
+      C.live h r.b)
+    (ensures fun h0 _ h1 ->
+      h0 == h1 /\
+      valid r h1)
+  = let h1 = get () in
+    let i = C.to_ibuffer r.b in
+    let aux (h:HS.mem)
+      : Lemma
+        (requires
+          valid r h /\
+          B.as_seq h i == B.as_seq h1 i)
+        (ensures
+          valid r h1)
+        [SMTPat (valid r h)]
+      = let m = r.meta in
+        LP.valid_ext_intro m.parser h (slice_of_ptr r) 0ul h1 (slice_of_ptr r) 0ul
+     in
+     let es =
+       let m = r.meta in
+       Ghost.hide m.repr_bytes
+     in
+     I.recall_value i es
+     
+module D = LowStar.Native.DynamicRegion
+
+(*
+ * Unlike other allocation functions in this module,
+ *   this function (and other flavors of alloc_and_blit) don't provide the witnessed contents
+ *   as the refinement of the return type
+ * This is because the contents depend on the input memory (== the contents of src)
+ *)
+let ralloc_and_blit (r:D.drgn) (src:C.const_buffer LP.byte) (len:U32.t)
+  : ST (b:C.const_buffer LP.byte)
+    (requires fun h0 ->
+      HS.live_region h0 (D.rid_of_drgn r) /\
+      U32.v len == C.length src /\
+      C.live h0 src)
+    (ensures fun h0 b h1 ->
+      let c = C.as_qbuf b in
+      let s = Seq.slice (C.as_seq h0 src) 0 (U32.v len) in
+      C.qbuf_qual c == C.IMMUTABLE /\
+      B.alloc_post_mem_common (C.to_ibuffer b) h0 h1 s /\
+      C.to_ibuffer b `I.value_is` s /\
+      D.region_lifetime_buf r (C.cast b) /\
+      B.frameOf (C.cast b) == (D.rid_of_drgn r))
+  = let src_buf = C.cast src in
+    let b : I.ibuffer LP.byte = D.ralloc_and_blit_buf r src_buf 0ul len in
+    let h0 = get() in
+    B.witness_p b (I.seq_eq (Ghost.hide (Seq.slice (B.as_seq h0 src_buf) 0 (U32.v len))));
+    C.of_ibuffer b
+
+
+/// `stash`: Main stateful operation
+///    Copies a ptr into a fresh stable ptr in the given region
+let stash (rgn:D.drgn) #t (r:ptr t) (len:uint_32{len > 0ul /\ len == r.meta.len /\ len < LP.validator_max_length}) 
+          #k (#p:LP.parser k t) (q:LS.parser32 p { k == r.meta.parser_kind /\ p == r.meta.parser /\ q == r.meta.parser32 })
+  : ST (r':stable_ptr t)
+   (requires fun h ->
+     valid r h /\
+     HS.live_region h (D.rid_of_drgn rgn))
+   (ensures fun h0 r' h1 ->
+     B.modifies B.loc_none h0 h1 /\
+     valid r' h1 /\
+     r.meta == r'.meta /\
+     D.region_lifetime_buf rgn (C.cast r'.b) /\
+     B.frameOf (C.cast r'.b) == (D.rid_of_drgn rgn))
+ = let buf' = ralloc_and_blit rgn r.b len in
+   let s = MkSlice buf' len in
+   let h = get () in
+   let _ = 
+     let slice = slice_of_const_buffer r.b len in
+     let slice' = slice_of_const_buffer buf' len in
+     LP.valid_facts r.meta.parser h slice 0ul; //elim valid_pos slice
+     LP.valid_facts r.meta.parser h slice' 0ul //intro valid_pos slice'
+   in
+   let p = {
+     b = buf';
+     meta = r.meta;
+     value = r.value;
+     ptr_ok = ()
+   } in
+   valid_if_live_intro p h;
+   p
